\documentclass[a4]{article}

\usepackage[utf8]{inputenc}

\usepackage{mathpartir}

\title{Règles d'inference}

\newcommand{\judg}[3]{#1 \vdash #2 : #3}
\newcommand{\G}{\Gamma}

\begin{document}

\maketitle

\begin{mathpar}
	\infer
	{ }
	{\judg \G {int} m}
	
	\infer
	{ }
	{\judg \G {bool} m}
	
	\infer
	{ }
	{\judg \G {char} m}
	
	\infer
	{ }
	{\judg \G {float} m}
\end{mathpar}

\begin{mathpar}
	\infer
	{{Def; \judg \G A m.ind}
	\\
	{Def; \judg \G B m.ind}}
	{\judg \G {A \rightarrow B} m}
	
	\infer
	{{Def; \judg \G A m.ind}
	\\
	{Def; \judg \G B m.ind}}
	{\judg \G {A \times B} m}
\end{mathpar}

\begin{mathpar}
	\infer
	{{(type (\alpha _i : \_) ^ I t) \in Def}
	\\
	{\judg \G {T[\alpha _i : A _i] ^ I} m}}
	{Def;\judg \G {(A _i) ^ I t} m}
\end{mathpar}

\begin{mathpar}
	\infer
	{{(type (\alpha _i : \_) t = (K _j \hspace{0.3em} of \hspace{0.3em} (A _i) ^{I _j}) ^J) \in Def}
	\\
	{\forall j \in J, \judg \G {K _j[\alpha _i : A _i] ^{I _j}} m}}
	{\judg \G {(A _i) ^ I t} m}
\end{mathpar}

\begin{mathpar}
	\infer
	{{(type(\alpha _i : m _i) ^I t) \in Def}
	\\
	{\forall i \in I, \judg \G {A _i} sep.m _i}}
	{Def;\judg \G {(A _i) ^ I t} m}	
\end{mathpar}

\iffalse
\begin{mathpar}
	\infer
	{{(type (\alpha _i : m _i) ^I u= U) \in Def}
	\\
	{(type (\beta _j : n _j) ^J t = \_) \in Def}
	\\
	{((A _i) ^{I _j} t) \in U}
	\\
	{\forall i \in (I _j) \G \vdash m _i = n _{f(i)}}}
	{Def; \judg \G {(B _j) ^J t} sep \Rightarrow (A _i) ^I u : sep}
\end{mathpar}
\fi

%		  (type (αᵢ : mᵢ) tᵢ = _ : m) ∈ Def
%  ∀i, Def; Γ ⊢ Aᵢ : mᵢ
%  ————————————————————
%  Def; Γ ⊢ (Aᵢ) tᵢ : m

\begin{mathpar}
	\infer
	{{Def = (type (\alpha _i : m _i) ^I t _j = T _j : m _j) ^J}
	\\
	{\forall j, Def; (\alpha _i : m _i) ^I \vdash T _j : m _j}}
	{\vdash Def}
\end{mathpar}

\begin{mathpar}
	\infer
	{{(type (\alpha _i : m _i) t _i = \_ : m) \in Def}
	\\
	{\forall i, Def; \judg \G (A _i) t _i : m _i}}
	{Def; \G \vdash (A _i) t _i : m}
\end{mathpar}

\begin{mathpar}
	\infer
	{Def; \G, \alpha : ind \vdash T:m}
	{Def; \judg \G {\exists \alpha , T} m}
\end{mathpar}

\iffalse
\begin{mathpar}
	\infer
	{{U _j = (\beta _i) ^ I t \in u}}
	{\judg \G {(A _i) ^ I t} sep \Rightarrow A _i : sep \Rightarrow B _i : sep}
	
	\infer
	{{T _j \neq (\beta _i) ^ I u \in t}}
	{\judg \G {(A _i) ^ I t} sep \Rightarrow (A _i) ^ I t' = T _j : sep}
\end{mathpar}
\fi

\end{document}